MMapGenTree.v
@@ -1,0 +1,830 @@
+(** * MSetGenTree : maps via generic trees
+
+    This module factorizes common parts in implementations
+    of finite maps as AVL trees and as Red-Black trees. The nodes
+    of the trees defined here include an generic information
+    parameter, that will be the height in AVL trees and the color
+    in Red-Black trees. Without more details here about these
+    information parameters, trees here are not known to be
+    well-balanced, but simply binary-search-trees.
+
+    The operations we could define and prove correct here are the
+    one that do not build non-empty trees, but only analyze them :
+
+     - empty is_empty
+     - find mem
+     - equal
+     - fold cardinal bindings
+*)
+
+Require Import Bool PeanoNat BinInt FunInd MMapInterface MMapList.
+Require Import Orders OrdersFacts OrdersLists.
+Local Open Scope list_scope.
+Local Open Scope lazy_bool_scope.
+
+Local Set Implicit Arguments.
+Local Unset Strict Implicit.
+
+(* For nicer extraction, we create induction principles
+   only when needed *)
+Local Unset Elimination Schemes.
+
+Module Type InfoTyp.
+ Parameter t : Set.
+End InfoTyp.
+
+(** * Ops : the pure functions *)
+
+Module Type Ops (X:OrderedType)(Info:InfoTyp).
+
+Definition key := X.t.
+Hint Transparent key.
+
+Section Elt.
+
+Variable elt : Type.
+
+(** * Trees *)
+
+Inductive tree  : Type :=
+| Leaf : tree
+| Node : Info.t -> tree -> X.t -> elt -> tree -> tree.
+
+Notation t := tree.
+
+(** ** The empty map and emptyness test *)
+
+Definition empty := Leaf.
+
+Definition is_empty t :=
+ match t with
+ | Leaf => true
+ | _ => false
+ end.
+
+(** ** Membership test *)
+
+(** The [mem] function is deciding membership. It exploits the
+    binary search tree invariant to achieve logarithmic complexity. *)
+
+Fixpoint mem x t :=
+ match t with
+ | Leaf => false
+ | Node _ l k _ r =>
+   match X.compare x k with
+     | Lt => mem x l
+     | Eq => true
+     | Gt => mem x r
+   end
+ end.
+
+Fixpoint find x m : option elt :=
+  match m with
+    |  Leaf => None
+    |  Node _ l y v r =>
+       match X.compare x y with
+         | Eq => Some v
+         | Lt => find x l
+         | Gt => find x r
+       end
+   end.
+
+(** ** Minimal, maximal, arbitrary bindings *)
+
+Fixpoint min_binding (t : tree) : option (key * elt) :=
+ match t with
+ | Leaf => None
+ | Node _ Leaf x e r => Some (x,e)
+ | Node _ l x e r => min_binding l
+ end.
+
+Fixpoint max_binding (t : tree) : option (key * elt) :=
+  match t with
+  | Leaf => None
+  | Node _ l x e Leaf => Some (x,e)
+  | Node _ l x e r => max_binding r
+  end.
+
+Definition choose := min_binding.
+
+(** ** Iteration on elements *)
+
+Fixpoint fold {A: Type} (f: key -> elt -> A -> A) (t: tree) (base: A) : A :=
+  match t with
+  | Leaf => base
+  | Node _ l x e r => fold f r (f x e (fold f l base))
+ end.
+
+Fixpoint bindings_aux acc s :=
+  match s with
+   | Leaf => acc
+   | Node _ l x e r => bindings_aux ((x,e) :: bindings_aux acc r) l
+  end.
+
+Definition bindings := bindings_aux nil.
+
+Fixpoint rev_bindings_aux acc s :=
+  match s with
+   | Leaf => acc
+   | Node _ l x e r => rev_bindings_aux ((x,e) :: rev_bindings_aux acc l) r
+  end.
+
+Definition rev_bindings := rev_bindings_aux nil.
+
+Fixpoint cardinal (s : tree) : nat :=
+  match s with
+   | Leaf => 0
+   | Node _ l _ _ r => S (cardinal l + cardinal r)
+  end.
+
+Fixpoint maxdepth s :=
+ match s with
+ | Leaf => 0
+ | Node _ l _ _ r => S (max (maxdepth l) (maxdepth r))
+ end.
+
+Fixpoint mindepth s :=
+ match s with
+ | Leaf => 0
+ | Node _ l _ _ r => S (min (mindepth l) (mindepth r))
+ end.
+
+(** ** Testing universal or existential properties. *)
+
+(** We do not use the standard boolean operators of Coq,
+    but lazy ones. *)
+
+Fixpoint for_all (f:key->elt->bool) s := match s with
+  | Leaf => true
+  | Node _ l x e r => f x e &&& for_all f l &&& for_all f r
+end.
+
+Fixpoint exists_ (f:key->elt->bool) s := match s with
+  | Leaf => false
+  | Node _ l x e r => f x e ||| exists_ f l ||| exists_ f r
+end.
+
+(** ** Comparison of trees *)
+
+(** The algorithm here has been suggested by Xavier Leroy,
+    and transformed into c.p.s. by Benjamin Grégoire.
+    The original ocaml code (with non-structural recursive calls)
+    has also been formalized (thanks to Function+measure), see
+    [ocaml_compare] in [MSetFullAVL]. The following code with
+    continuations computes dramatically faster in Coq, and
+    should be almost as efficient after extraction.
+*)
+
+(** * Comparison *)
+
+Variable cmp : elt->elt->bool.
+
+(** Enumeration of the elements of a tree. This corresponds
+    to the "samefringe" notion in the litterature. *)
+
+Inductive enumeration :=
+ | End : enumeration
+ | More : key -> elt -> tree -> enumeration -> enumeration.
+
+(** [cons t e] adds the elements of tree [t] on the head of
+    enumeration [e]. *)
+
+Fixpoint cons s e : enumeration :=
+ match s with
+  | Leaf => e
+  | Node _ l x v r => cons l (More x v r e)
+ end.
+
+(** One step of comparison of elements *)
+
+Definition equal_more x1 v1 (cont:enumeration->bool) e2 :=
+ match e2 with
+ | End => false
+ | More x2 v2 r2 e2 =>
+     match X.compare x1 x2 with
+      | Eq => cmp v1 v2 &&& cont (cons r2 e2)
+      | _ => false
+     end
+ end.
+
+(** Comparison of left tree, middle element, then right tree *)
+
+Fixpoint equal_cont m1 (cont:enumeration->bool) e2 :=
+ match m1 with
+  | Leaf => cont e2
+  | Node _ l1 x1 v1 r1 =>
+     equal_cont l1 (equal_more x1 v1 (equal_cont r1 cont)) e2
+  end.
+
+(** Initial continuation *)
+
+Definition equal_end e2 := match e2 with End => true | _ => false end.
+
+(** The complete comparison *)
+
+Definition equal m1 m2 := equal_cont m1 equal_end (cons m2 End).
+
+End Elt.
+Notation t := tree.
+End Ops.
+
+(** * Props : correctness proofs of these generic operations *)
+
+Module Type Props (X:OrderedType)(Info:InfoTyp)(Import M:Ops X Info).
+
+Section Invariants.
+Variable elt : Type.
+
+(** ** Occurrence in a tree *)
+
+Inductive MapsTo (x : key)(e : elt) : t elt -> Prop :=
+  | MapsRoot : forall l r h y,
+      X.eq x y -> MapsTo x e (Node h l y e r)
+  | MapsLeft : forall l r h y e',
+      MapsTo x e l -> MapsTo x e (Node h l y e' r)
+  | MapsRight : forall l r h y e',
+      MapsTo x e r -> MapsTo x e (Node h l y e' r).
+
+Inductive In (x : key) : t elt -> Prop :=
+  | InRoot : forall l r h y e,
+      X.eq x y -> In x (Node h l y e r)
+  | InLeft : forall l r h y e',
+      In x l -> In x (Node h l y e' r)
+  | InRight : forall l r h y e',
+      In x r -> In x (Node h l y e' r).
+
+Definition In0 k m := exists e:elt, MapsTo k e m.
+
+(** ** Binary search trees *)
+
+(** [Above x m] : [x] is strictly greater than any key in [m].
+    [Below x m] : [x] is strictly smaller than any key in [m]. *)
+
+Inductive Above (x:key) : t elt -> Prop :=
+ | AbLeaf : Above x (Leaf _)
+ | AbNode l r h y e : Above x l -> X.lt y x -> Above x r ->
+   Above x (Node h l y e r).
+
+Inductive Below (x:key) : t elt -> Prop :=
+ | BeLeaf : Below x (Leaf _)
+ | BeNode l r h y e : Below x l -> X.lt x y -> Below x r ->
+   Below x (Node h l y e r).
+
+Definition Apart (m1 m2 : t elt) : Prop :=
+  forall x1 x2, In x1 m1 -> In x2 m2 -> X.lt x1 x2.
+
+(** Alternative statements, equivalent with [LtTree] and [GtTree] *)
+
+Definition lt_tree x m := forall y, In y m -> X.lt y x.
+Definition gt_tree x m := forall y, In y m -> X.lt x y.
+
+(** [Bst t] : [t] is a binary search tree *)
+
+Inductive Bst : t elt -> Prop :=
+  | BSLeaf : Bst (Leaf _)
+  | BSNode : forall h x e l r, Bst l -> Bst r ->
+     Above x l -> Below x r -> Bst (Node h l x e r).
+
+End Invariants.
+
+Module MX := OrderedTypeFacts X.
+Module PX := KeyOrderedType X.
+Module L := MMapList.Raw X.
+
+Local Infix "∈" := In (at level 70).
+Local Infix "==" := X.eq (at level 70).
+Local Infix "<" := X.lt (at level 70).
+Local Infix "<<" := Below (at level 70).
+Local Infix ">>" := Above (at level 70).
+Local Infix "<<<" := Apart (at level 70).
+
+Scheme tree_ind := Induction for tree Sort Prop.
+Scheme Bst_ind := Induction for Bst Sort Prop.
+Scheme MapsTo_ind := Induction for MapsTo Sort Prop.
+Scheme In_ind := Induction for In Sort Prop.
+Scheme Above_ind := Induction for Above Sort Prop.
+Scheme Below_ind := Induction for Below Sort Prop.
+
+Functional Scheme mem_ind := Induction for mem Sort Prop.
+Functional Scheme find_ind := Induction for find Sort Prop.
+
+(** * Automation and dedicated tactics. *)
+
+Local Hint Constructors tree MapsTo In Bst Above Below.
+Local Hint Unfold lt_tree gt_tree Apart.
+Local Hint Immediate MX.eq_sym.
+Local Hint Resolve MX.eq_refl MX.eq_trans MX.lt_trans.
+
+Tactic Notation "factornode" ident(s) :=
+ try clear s;
+ match goal with
+   | |- context [Node ?h ?l ?x ?e ?r] =>
+       set (s:=Node h l x e r) in *; clearbody s; clear l x e r h
+   | _ : context [Node ?h ?l ?x ?e ?r] |- _ =>
+       set (s:=Node h l x e r) in *; clearbody s; clear l x e r h
+ end.
+
+(** A tactic for cleaning hypothesis after use of functional induction. *)
+
+Ltac cleanf :=
+ match goal with
+  | H : X.compare _ _ = Eq |- _ =>
+    rewrite ?H; apply MX.compare_eq in H; cleanf
+  | H : X.compare _ _ = Lt |- _ =>
+    rewrite ?H; apply MX.compare_lt_iff in H; cleanf
+  | H : X.compare _ _ = Gt |- _ =>
+    rewrite ?H; apply MX.compare_gt_iff in H; cleanf
+  | _ => idtac
+ end.
+
+
+(** A tactic to repeat [inversion_clear] on all hyps of the
+    form [(f (Node ...))] *)
+
+Ltac inv f :=
+  match goal with
+     | H:f (Leaf _) |- _ => inversion_clear H; inv f
+     | H:f _ (Leaf _) |- _ => inversion_clear H; inv f
+     | H:f _ _ (Leaf _) |- _ => inversion_clear H; inv f
+     | H:f _ _ _ (Leaf _) |- _ => inversion_clear H; inv f
+     | H:f (Node _ _ _ _ _) |- _ => inversion_clear H; inv f
+     | H:f _ (Node _ _ _ _ _) |- _ => inversion_clear H; inv f
+     | H:f _ _ (Node _ _ _ _ _) |- _ => inversion_clear H; inv f
+     | H:f _ _ _ (Node _ _ _ _ _) |- _ => inversion_clear H; inv f
+     | _ => idtac
+  end.
+
+Ltac inv_all f :=
+  match goal with
+   | H: f _ |- _ => inversion_clear H; inv f
+   | H: f _ _ |- _ => inversion_clear H; inv f
+   | H: f _ _ _ |- _ => inversion_clear H; inv f
+   | H: f _ _ _ _ |- _ => inversion_clear H; inv f
+   | _ => idtac
+  end.
+
+Ltac intuition_in := repeat (intuition; inv In; inv MapsTo).
+
+(** * Basic results about [MapsTo], [In], [lt_tree], [gt_tree], [height] *)
+
+(** Facts about [MapsTo] and [In]. *)
+
+Lemma MapsTo_In {elt} k (e:elt) m : MapsTo k e m -> k ∈ m.
+Proof.
+ induction 1; auto.
+Qed.
+Local Hint Resolve MapsTo_In.
+
+Lemma In_MapsTo {elt} k m : k ∈ m -> exists (e:elt), MapsTo k e m.
+Proof.
+ induction 1; try destruct IHIn as (e,He); exists e; auto.
+Qed.
+
+Lemma In_alt {elt} k (m:t elt) : In0 k m <-> k ∈ m.
+Proof.
+ split.
+ intros (e,H); eauto.
+ unfold In0; apply In_MapsTo; auto.
+Qed.
+
+Lemma MapsTo_1 {elt} m x y (e:elt) :
+  x == y -> MapsTo x e m -> MapsTo y e m.
+Proof.
+ induction m; simpl; intuition_in; eauto.
+Qed.
+Hint Immediate MapsTo_1.
+
+Instance MapsTo_compat {elt} :
+  Proper (X.eq==>Logic.eq==>Logic.eq==>iff) (@MapsTo elt).
+Proof.
+ intros x x' Hx e e' He m m' Hm. subst.
+ split; now apply MapsTo_1.
+Qed.
+
+Instance In_compat {elt} :
+  Proper (X.eq==>Logic.eq==>iff) (@In elt).
+Proof.
+ intros x x' H m m' <-.
+ induction m; simpl; intuition_in; eauto.
+Qed.
+
+Lemma In_node_iff {elt} l x (e:elt) r h y :
+  y ∈ (Node h l x e r) <-> y ∈ l \/ y == x \/ y ∈ r.
+Proof.
+ intuition_in.
+Qed.
+
+(** Results about [Above] and [Below] *)
+
+Lemma above {elt} (m:t elt) x :
+  x >> m <-> forall y, y ∈ m -> y < x.
+Proof.
+ split.
+ - induction 1; intuition_in; MX.order.
+ - induction m; constructor; auto.
+Qed.
+
+Lemma below {elt} (m:t elt) x :
+  x << m <-> forall y, y ∈ m -> x < y.
+Proof.
+ split.
+ - induction 1; intuition_in; MX.order.
+ - induction m; constructor; auto.
+Qed.
+
+Lemma AboveLt {elt} (m:t elt) x y : x >> m -> y ∈ m -> y < x.
+Proof.
+ rewrite above; intuition.
+Qed.
+
+Lemma BelowGt {elt} (m:t elt) x y : x << m -> y ∈ m -> x < y.
+Proof.
+ rewrite below; intuition.
+Qed.
+
+Lemma Above_not_In {elt} (m:t elt) x : x >> m -> ~ x ∈ m.
+Proof.
+ induction 1; intuition_in; MX.order.
+Qed.
+
+Lemma Below_not_In {elt} (m:t elt) x : x << m -> ~ x ∈ m.
+Proof.
+ induction 1; intuition_in; MX.order.
+Qed.
+
+Lemma Above_trans {elt} (m:t elt) x y : x < y -> x >> m -> y >> m.
+Proof.
+ induction 2; constructor; trivial; MX.order.
+Qed.
+
+Lemma Below_trans {elt} (m:t elt) x y : y < x -> x << m -> y << m.
+Proof.
+ induction 2; constructor; trivial; MX.order.
+Qed.
+
+Local Hint Resolve
+ AboveLt Above_not_In Above_trans
+ BelowGt Below_not_In Below_trans.
+
+(** Helper tactic concerning order of elements. *)
+
+Ltac order := match goal with
+ | U: _ >> ?m, V: _ ∈ ?m |- _ =>
+   generalize (AboveLt U V); clear U; order
+ | U: _ << ?m, V: _ ∈ ?m |- _ =>
+   generalize (BelowGt U V); clear U; order
+ | U: _ >> ?m, V: MapsTo _ _ ?m |- _ =>
+   generalize (AboveLt U (MapsTo_In V)); clear U; order
+ | U: _ << ?m, V: MapsTo _ _ ?m |- _ =>
+   generalize (BelowGt U (MapsTo_In V)); clear U; order
+ | _ => MX.order
+end.
+
+Lemma between {elt} (m m':t elt) x :
+  x >> m -> x << m' -> m <<< m'.
+Proof.
+ intros H H' y y' Hy Hy'. order.
+Qed.
+
+Section Elt.
+Variable elt:Type.
+Implicit Types m r : t elt.
+
+(** * Membership *)
+
+Lemma find_1 m x e : Bst m -> MapsTo x e m -> find x m = Some e.
+Proof.
+ functional induction (find x m); cleanf;
+  intros; inv Bst; intuition_in; order.
+Qed.
+
+Lemma find_2 m x e : find x m = Some e -> MapsTo x e m.
+Proof.
+ functional induction (find x m); cleanf; subst; intros; auto.
+ - discriminate.
+ - injection H as ->. auto.
+Qed.
+
+Lemma find_spec m x e : Bst m ->
+ (find x m = Some e <-> MapsTo x e m).
+Proof.
+ split; auto using find_1, find_2.
+Qed.
+
+Lemma find_in m x : find x m <> None -> x ∈ m.
+Proof.
+ destruct (find x m) eqn:F; intros H.
+ - apply MapsTo_In with e. now apply find_2.
+ - now elim H.
+Qed.
+
+Lemma in_find m x : Bst m -> x ∈ m -> find x m <> None.
+Proof.
+ intros H H'.
+ destruct (In_MapsTo H') as (d,Hd).
+ now rewrite (find_1 H Hd).
+Qed.
+
+Lemma find_in_iff m x : Bst m ->
+ (find x m <> None <-> x ∈ m).
+Proof.
+ split; auto using find_in, in_find.
+Qed.
+
+Lemma not_find_iff m x : Bst m ->
+ (find x m = None <-> ~ x ∈ m).
+Proof.
+ intros H. rewrite <- find_in_iff; trivial.
+ destruct (find x m); split; try easy. now destruct 1.
+Qed.
+
+Lemma eq_option_alt (o o':option elt) :
+ o=o' <-> (forall e, o=Some e <-> o'=Some e).
+Proof.
+split; intros.
+- now subst.
+- destruct o, o'; rewrite ?H; auto. symmetry; now apply H.
+Qed.
+
+Lemma find_mapsto_equiv : forall m m' x, Bst m -> Bst m' ->
+ (find x m = find x m' <->
+  (forall d, MapsTo x d m <-> MapsTo x d m')).
+Proof.
+ intros m m' x Hm Hm'. rewrite eq_option_alt.
+ split; intros H d. now rewrite <- 2 find_spec. now rewrite 2 find_spec.
+Qed.
+
+Lemma find_in_equiv : forall m m' x, Bst m -> Bst m' ->
+ find x m = find x m' ->
+ (x ∈ m <-> x ∈ m').
+Proof.
+ split; intros; apply find_in; [ rewrite <- H1 | rewrite H1 ];
+  apply in_find; auto.
+Qed.
+
+Lemma find_compat m x x' : Bst m -> X.eq x x' -> find x m = find x' m.
+Proof.
+  intros B E.
+  destruct (find x' m) eqn:H.
+  - apply find_1; trivial. rewrite E. now apply find_2.
+  - rewrite not_find_iff in *; trivial. now rewrite E.
+Qed.
+
+Lemma mem_spec m x : Bst m -> mem x m = true <-> x ∈ m.
+Proof.
+ functional induction (mem x m); auto; intros; cleanf;
+  inv Bst; intuition_in; try discriminate; order.
+Qed.
+
+(** * Empty map *)
+
+Lemma empty_bst : Bst (empty elt).
+Proof.
+ constructor.
+Qed.
+
+Lemma empty_spec x : find x (empty elt) = None.
+Proof.
+ reflexivity.
+Qed.
+
+(** * Emptyness test *)
+
+Lemma is_empty_spec m : is_empty m = true <-> forall x, find x m = None.
+Proof.
+ destruct m as [|h r x e l]; simpl; split; try easy.
+ intros H. specialize (H x). now rewrite MX.compare_refl in H.
+Qed.
+
+(** * Elements *)
+
+Notation eqk := (PX.eqk (elt:= elt)).
+Notation eqke := (PX.eqke (elt:= elt)).
+Notation ltk := (PX.ltk (elt:= elt)).
+
+Lemma bindings_aux_mapsto : forall (s:t elt) acc x e,
+ InA eqke (x,e) (bindings_aux acc s) <-> MapsTo x e s \/ InA eqke (x,e) acc.
+Proof.
+ induction s as [ | h l Hl x e r Hr ]; simpl; auto.
+ intuition.
+ inversion H0.
+ intros.
+ rewrite Hl.
+ destruct (Hr acc x0 e0); clear Hl Hr.
+ intuition; inversion_clear H3; intuition.
+ compute in H0. destruct H0; simpl in *; subst; intuition.
+Qed.
+
+Lemma bindings_mapsto : forall (s:t elt) x e,
+ InA eqke (x,e) (bindings s) <-> MapsTo x e s.
+Proof.
+ intros; generalize (bindings_aux_mapsto s nil x e); intuition.
+ inversion_clear H0.
+Qed.
+
+Lemma bindings_in : forall (s:t elt) x, L.PX.In x (bindings s) <-> x ∈ s.
+Proof.
+ intros.
+ unfold L.PX.In.
+ rewrite <- In_alt; unfold In0.
+ split; intros (y,H); exists y.
+ - now rewrite <- bindings_mapsto.
+ - unfold L.PX.MapsTo; now rewrite bindings_mapsto.
+Qed.
+
+Lemma bindings_aux_sort : forall (s:t elt) acc,
+ Bst s -> sort ltk acc ->
+ (forall x e y, InA eqke (x,e) acc -> y ∈ s -> y < x) ->
+ sort ltk (bindings_aux acc s).
+Proof.
+ induction s as [ | h l Hl y e r Hr ]; simpl; intuition.
+ inv Bst.
+ apply Hl; auto.
+ - constructor.
+   + apply Hr; eauto.
+   + clear Hl Hr.
+     apply InA_InfA with (eqA:=eqke); auto with *.
+     intros (y',e') Hy'.
+     apply bindings_aux_mapsto in Hy'. compute. intuition; eauto.
+ - clear Hl Hr. intros x e' y' Hx Hy'.
+   inversion_clear Hx.
+   + compute in H. destruct H; simpl in *. order.
+   + apply bindings_aux_mapsto in H. intuition eauto.
+Qed.
+
+Lemma bindings_sort : forall s : t elt, Bst s -> sort ltk (bindings s).
+Proof.
+ intros; unfold bindings; apply bindings_aux_sort; auto.
+ intros; inversion H0.
+Qed.
+Hint Resolve bindings_sort.
+
+Lemma bindings_nodup : forall s : t elt, Bst s -> NoDupA eqk (bindings s).
+Proof.
+ intros; apply PX.Sort_NoDupA; auto.
+Qed.
+
+Lemma bindings_aux_cardinal m acc :
+ (length acc + cardinal m)%nat = length (bindings_aux acc m).
+Proof.
+ revert acc. induction m; simpl; intuition.
+ rewrite <- IHm1; simpl.
+ rewrite <- IHm2. rewrite Nat.add_succ_r, <- Nat.add_assoc.
+ f_equal. f_equal. apply Nat.add_comm.
+Qed.
+
+Lemma bindings_cardinal m : cardinal m = length (bindings m).
+Proof.
+ exact (bindings_aux_cardinal m nil).
+Qed.
+
+Lemma bindings_app :
+ forall (s:t elt) acc, bindings_aux acc s = bindings s ++ acc.
+Proof.
+ induction s; simpl; intros; auto.
+ rewrite IHs1, IHs2.
+ unfold bindings; simpl.
+ rewrite 2 IHs1, IHs2, !app_nil_r, !app_ass; auto.
+Qed.
+
+Lemma bindings_node :
+ forall (t1 t2:t elt) x e z l,
+ bindings t1 ++ (x,e) :: bindings t2 ++ l =
+ bindings (Node z t1 x e t2) ++ l.
+Proof.
+ unfold bindings; simpl; intros.
+ rewrite !bindings_app, !app_nil_r, !app_ass; auto.
+Qed.
+
+(** * Fold *)
+
+Definition fold' {A} (f : key -> elt -> A -> A)(s : t elt) :=
+  L.fold f (bindings s).
+
+Lemma fold_equiv_aux {A} (s : t elt) (f : key -> elt -> A -> A) (a : A) acc :
+ L.fold f (bindings_aux acc s) a = L.fold f acc (fold f s a).
+Proof.
+ revert a acc.
+ induction s; simpl; trivial.
+ intros. rewrite IHs1. simpl. apply IHs2.
+Qed.
+
+Lemma fold_equiv {A} (s : t elt) (f : key -> elt -> A -> A) (a : A) :
+ fold f s a = fold' f s a.
+Proof.
+ unfold fold', bindings. now rewrite fold_equiv_aux.
+Qed.
+
+Lemma fold_spec (s:t elt)(Hs:Bst s){A}(i:A)(f : key -> elt -> A -> A) :
+ fold f s i = fold_left (fun a p => f (fst p) (snd p) a) (bindings s) i.
+Proof.
+ rewrite fold_equiv. unfold fold'. now rewrite L.fold_spec.
+Qed.
+
+(** * Comparison *)
+
+(** [flatten_e e] returns the list of bindings of the enumeration [e]
+    i.e. the list of bindings actually compared *)
+
+Fixpoint flatten_e (e : enumeration elt) : list (key*elt) := match e with
+  | End _ => nil
+  | More x e t r => (x,e) :: bindings t ++ flatten_e r
+ end.
+
+Lemma flatten_e_bindings :
+ forall (l:t elt) r x d z e,
+ bindings l ++ flatten_e (More x d r e) =
+ bindings (Node z l x d r) ++ flatten_e e.
+Proof.
+ intros; apply bindings_node.
+Qed.
+
+Lemma cons_1 : forall (s:t elt) e,
+  flatten_e (cons s e) = bindings s ++ flatten_e e.
+Proof.
+  induction s; auto; intros.
+  simpl flatten_e; rewrite IHs1; apply flatten_e_bindings; auto.
+Qed.
+
+(** Proof of correction for the comparison *)
+
+Variable cmp : elt->elt->bool.
+
+Definition IfEq b l1 l2 := L.equal cmp l1 l2 = b.
+
+Lemma cons_IfEq : forall b x1 x2 d1 d2 l1 l2,
+  X.eq x1 x2 -> cmp d1 d2 = true ->
+  IfEq b l1 l2 ->
+    IfEq b ((x1,d1)::l1) ((x2,d2)::l2).
+Proof.
+ unfold IfEq; destruct b; simpl; intros; case X.compare_spec; simpl;
+  try rewrite H0; auto; order.
+Qed.
+
+Lemma equal_end_IfEq : forall e2,
+  IfEq (equal_end e2) nil (flatten_e e2).
+Proof.
+ destruct e2; red; auto.
+Qed.
+
+Lemma equal_more_IfEq :
+ forall x1 d1 (cont:enumeration elt -> bool) x2 d2 r2 e2 l,
+  IfEq (cont (cons r2 e2)) l (bindings r2 ++ flatten_e e2) ->
+    IfEq (equal_more cmp x1 d1 cont (More x2 d2 r2 e2)) ((x1,d1)::l)
+       (flatten_e (More x2 d2 r2 e2)).
+Proof.
+ unfold IfEq; simpl; intros; destruct X.compare; simpl; auto.
+ rewrite <-andb_lazy_alt; f_equal; auto.
+Qed.
+
+Lemma equal_cont_IfEq : forall m1 cont e2 l,
+  (forall e, IfEq (cont e) l (flatten_e e)) ->
+  IfEq (equal_cont cmp m1 cont e2) (bindings m1 ++ l) (flatten_e e2).
+Proof.
+ induction m1 as [|h1 l1 Hl1 x1 d1 r1 Hr1]; intros; auto.
+ rewrite <- bindings_node; simpl.
+ apply Hl1; auto.
+ clear e2; intros [|x2 d2 r2 e2].
+ simpl; red; auto.
+ apply equal_more_IfEq.
+ rewrite <- cons_1; auto.
+Qed.
+
+Lemma equal_IfEq : forall (m1 m2:t elt),
+  IfEq (equal cmp m1 m2) (bindings m1) (bindings m2).
+Proof.
+ intros; unfold equal.
+ rewrite <- (app_nil_r (bindings m1)).
+ replace (bindings m2) with (flatten_e (cons m2 (End _)))
+  by (rewrite cons_1; simpl; rewrite app_nil_r; auto).
+ apply equal_cont_IfEq.
+ intros.
+ apply equal_end_IfEq; auto.
+Qed.
+
+Definition Equivb m m' :=
+  (forall k, In k m <-> In k m') /\
+  (forall k e e', MapsTo k e m -> MapsTo k e' m' -> cmp e e' = true).
+
+Lemma Equivb_bindings : forall s s',
+ Equivb s s' <-> L.Equivb cmp (bindings s) (bindings s').
+Proof.
+unfold Equivb, L.Equivb; split; split; intros.
+do 2 rewrite bindings_in; firstorder.
+destruct H.
+apply (H2 k); rewrite <- bindings_mapsto; auto.
+do 2 rewrite <- bindings_in; firstorder.
+destruct H.
+apply (H2 k); unfold L.PX.MapsTo; rewrite bindings_mapsto; auto.
+Qed.
+
+Lemma equal_Equivb : forall (s s': t elt), Bst s -> Bst s' ->
+  (equal cmp s s' = true <-> Equivb s s').
+Proof.
+ intros s s' B B'.
+ rewrite Equivb_bindings, <- equal_IfEq.
+ split; [apply L.equal_2|apply L.equal_1]; auto.
+Qed.
+
+End Elt.
+End Props.
